more ground superposition

Weidenbach_Book/Propo_Superposition.thy
@@ -1,34 +1,38 @@
 theory Propo_Superposition
 imports Partial_Clausal_Logic "../lib/Herbrand_Interpretation"
 begin
+
 no_notation Herbrand_Interpretation.true_cls (infix "\<Turnstile>" 50)
 notation Herbrand_Interpretation.true_cls (infix "\<Turnstile>h" 50)
 
 no_notation Herbrand_Interpretation.true_cls (infix "\<Turnstile>s" 50)
 notation Herbrand_Interpretation.true_clss (infix "\<Turnstile>hs" 50)
 
-definition clss_lt :: "'a::wellorder clauses \<Rightarrow> 'a clause \<Rightarrow> 'a clauses" ("_\<^sup>\<prec>\<^sup>_") where
-"clss_lt N C = {D \<in> N. D #<# C}"
+lemma herbrand_interp_iff_partial_interp_cls:
+  "S \<Turnstile>h C \<longleftrightarrow> {Pos P|P. P\<in>S} \<union> {Neg P|P. P\<notin>S} \<Turnstile> C"
+  unfolding Herbrand_Interpretation.true_cls_def Partial_Clausal_Logic.true_cls_def
+  by auto
 
-definition abstract_red :: "'a::wellorder clause \<Rightarrow> 'a clauses \<Rightarrow> bool" where
-"abstract_red C N = (clss_lt N C \<Turnstile>p C)"
+lemma herbrand_consistent_interp:
+  "consistent_interp ({Pos P|P. P\<in>S} \<union> {Neg P|P. P\<notin>S})"
+  unfolding consistent_interp_def by auto
 
-lemma tautology_is_redundant:
-  assumes "tautology C"
-  shows "abstract_red C N"
-  using assms unfolding abstract_red_def true_clss_cls_def tautology_def by auto
-  
-lemma subsumed_is_redundant:
-  assumes AB: "A \<subset># B"
-  and AN: "A \<in> N" and "B \<in> N"
-  shows "abstract_red B N"
-proof -
-  have "A \<in> clss_lt N B" using AN AB unfolding clss_lt_def 
-    by (auto dest: less_eq_imp_le_multiset simp add: multiset_order.dual_order.order_iff_strict)
-  thus ?thesis
-    using AB unfolding abstract_red_def true_clss_cls_def Partial_Clausal_Logic.true_clss_def by blast
-qed
-  
+lemma herbrand_total_over_set:
+  "total_over_set ({Pos P|P. P\<in>S} \<union> {Neg P|P. P\<notin>S}) T"
+  unfolding total_over_set_def by auto
+
+lemma herbrand_total_over_m:
+  "total_over_m ({Pos P|P. P\<in>S} \<union> {Neg P|P. P\<notin>S}) T"
+  unfolding total_over_m_def by (auto simp add: herbrand_total_over_set)
+
+lemma herbrand_interp_iff_partial_interp_clss:
+  "S \<Turnstile>hs C \<longleftrightarrow> {Pos P|P. P\<in>S} \<union> {Neg P|P. P\<notin>S} \<Turnstile>s C"
+  unfolding true_clss_def Ball_def herbrand_interp_iff_partial_interp_cls
+  Partial_Clausal_Logic.true_clss_def by auto
+
+definition clss_lt :: "'a::wellorder clauses \<Rightarrow> 'a clause \<Rightarrow> 'a clauses" ("_<^bsup>\<^sup>_<^esup>") where
+"clss_lt N C = {D \<in> N. D #\<subset># C}"
+
 locale selection =
   fixes S :: "'a clause \<Rightarrow> 'a clause"
   assumes
@@ -48,11 +52,10 @@ function
   production :: "'a clause \<Rightarrow> 'a interp"
 where
   "production C =
-   {A. C \<in> N \<and> C \<noteq> {#} \<and> Max (set_mset C) = Pos A \<and> \<not> (\<Union>D \<in> {D. D #\<subset># C}. production D) \<Turnstile>h C \<and>
-      S C = {#}}"
+   {A. C \<in> N \<and> C \<noteq> {#} \<and> Max (set_mset C) = Pos A \<and> count C (Pos A) \<le> 1
+     \<and> \<not> (\<Union>D \<in> {D. D #\<subset># C}. production D) \<Turnstile>h C \<and> S C = {#}}"
   by auto
-  termination by (relation "{(D, C). D #\<subset># C}") (auto simp: wf_less_multiset)
-
+termination by (relation "{(D, C). D #\<subset># C}") (auto simp: wf_less_multiset)
 
 declare production.simps[simp del]
 
@@ -60,7 +63,7 @@ definition interp :: "'a clause \<Rightarrow> 'a interp" where
   "interp C = (\<Union>D \<in> {D. D #\<subset># C}. production D)"
 
 lemma production_unfold:
-  "production C = {A. C \<in> N \<and> C \<noteq> {#} \<and> Max (set_mset C) = Pos A \<and> \<not> interp C \<Turnstile>h C \<and> S C = {#}}"
+  "production C = {A. C \<in> N \<and> C \<noteq> {#} \<and> Max (set_mset C) = Pos A\<and> count C (Pos A) \<le> 1 \<and> \<not> interp C \<Turnstile>h C \<and> S C = {#}}"
   unfolding interp_def by (rule production.simps)
 
 abbreviation "productive A \<equiv> (production A \<noteq> {})"
@@ -69,7 +72,7 @@ abbreviation produces :: "'a clause \<Rightarrow> 'a \<Rightarrow> bool" where
   "produces C A \<equiv> production C = {A}"
 
 lemma producesD:
-  "produces C A \<Longrightarrow> C \<in> N \<and> C \<noteq> {#} \<and> Pos A = Max (set_mset C) \<and> \<not> interp C \<Turnstile>h C \<and> S C = {#}"
+  "produces C A \<Longrightarrow> C \<in> N \<and> C \<noteq> {#} \<and> Pos A = Max (set_mset C) \<and> count C (Pos A) \<le> 1\<and> \<not> interp C \<Turnstile>h C \<and> S C = {#}"
   unfolding production_unfold by auto
 
 lemma "produces C A \<Longrightarrow> Pos A \<in># C"
@@ -80,31 +83,473 @@ lemma interp'_def_in_set:
   unfolding interp_def apply auto
   unfolding production_unfold apply auto
   done
-end
 
-definition partial_model :: "'a clauses \<Rightarrow> 'a interp" ("_\<^sub>\<I>") where
-"partial_model N = (\<Union>D \<in> {D. D \<in>N}. production N D)"
+lemma production_iff_produces:
+  "produces D A \<longleftrightarrow> A \<in> production D"
+  unfolding production_unfold by auto
 
-lemma "partial_model {} =  {}"
-  unfolding partial_model_def by auto
-
-lemma
-  assumes D: "C+{#-P#} #\<subset># D" 
-  shows "ground_resolution_with_selection.production S N D \<noteq> {atm_of P}"
-oops
+definition Interp :: "'a clause \<Rightarrow> 'a interp" where
+  "Interp C = interp C \<union> production C"
 
 lemma
-  assumes "produces N C P"
-  shows "partial_model N \<Turnstile>h C"
-oops
+  assumes "produces C P"
+  shows "Interp C \<Turnstile>h C"
+  unfolding Interp_def assms using producesD[OF assms] 
+  by (metis Max_in_lits Un_insert_right insertI1 pos_literal_in_imp_true_cls)
+
+definition INTERP :: "'a interp" where
+"INTERP = (\<Union>D \<in>N. production D)"
+
+
+lemma interp_subseteq_Interp[simp]: "interp C \<subseteq> Interp C"
+  unfolding Interp_def by simp
+
+lemma Interp_as_UNION: "Interp C = (\<Union>D \<in> {D. D #\<subseteq># C}. production D)"
+  unfolding Interp_def interp_def le_multiset_def by fast
+
+lemma productive_not_empty: "productive C \<Longrightarrow> C \<noteq> {#}"
+  unfolding production_unfold by auto
+
+lemma productive_imp_produces_Max_literal: "productive C \<Longrightarrow> produces C (atm_of (Max (set_mset C)))"
+  unfolding production_unfold by (auto simp del: atm_of_Max_lit)
+
+lemma productive_imp_produces_Max_atom: "productive C \<Longrightarrow> produces C (Max (atms_of C))"
+  unfolding atms_of_def Max_atm_of_set_mset_commute[OF productive_not_empty]
+  by (rule productive_imp_produces_Max_literal)
+
+lemma produces_imp_Max_literal: "produces C A \<Longrightarrow> A = atm_of (Max (set_mset C))"
+  by (metis Max_singleton insert_not_empty productive_imp_produces_Max_literal)
+
+lemma produces_imp_Max_atom: "produces C A \<Longrightarrow> A = Max (atms_of C)"
+  by (metis Max_singleton insert_not_empty productive_imp_produces_Max_atom)
+
+lemma produces_imp_Pos_in_lits: "produces C A \<Longrightarrow> Pos A \<in># C"
+  by (auto intro: Max_in_lits dest!: producesD)
+
+lemma productive_in_N: "productive C \<Longrightarrow> C \<in> N"
+  unfolding production_unfold by auto
+
+lemma produces_imp_atms_leq: "produces C A \<Longrightarrow> B \<in> atms_of C \<Longrightarrow> B \<le> A"
+  by (metis Max_ge finite_atms_of insert_not_empty productive_imp_produces_Max_atom
+    singleton_inject)
+
+lemma produces_imp_neg_notin_lits: "produces C A \<Longrightarrow> \<not> Neg A \<in># C"
+  by (auto intro!: pos_Max_imp_neg_notin dest: producesD simp del: not_gr0)
+
+lemma less_eq_imp_interp_subseteq_interp: "C #\<subseteq># D \<Longrightarrow> interp C \<subseteq> interp D"
+  unfolding interp_def by auto (metis multiset_order.order.strict_trans2)
+
+lemma less_eq_imp_interp_subseteq_Interp: "C #\<subseteq># D \<Longrightarrow> interp C \<subseteq> Interp D"
+  unfolding Interp_def using less_eq_imp_interp_subseteq_interp by blast
+
+lemma less_imp_production_subseteq_interp: "C #\<subset># D \<Longrightarrow> production C \<subseteq> interp D"
+  unfolding interp_def by fast
+
+lemma less_eq_imp_production_subseteq_Interp: "C #\<subseteq># D \<Longrightarrow> production C \<subseteq> Interp D"
+  unfolding Interp_def using less_imp_production_subseteq_interp
+  by (metis multiset_order.le_imp_less_or_eq le_supI1 sup_ge2)
+
+lemma less_imp_Interp_subseteq_interp: "C #\<subset># D \<Longrightarrow> Interp C \<subseteq> interp D"
+  unfolding Interp_def
+  by (auto simp: less_eq_imp_interp_subseteq_interp less_imp_production_subseteq_interp)
+
+lemma less_eq_imp_Interp_subseteq_Interp: "C #\<subseteq># D \<Longrightarrow> Interp C \<subseteq> Interp D"
+  using less_imp_Interp_subseteq_interp
+  unfolding Interp_def by (metis multiset_order.le_imp_less_or_eq le_supI2 subset_refl sup_commute)
+
+lemma false_Interp_to_true_interp_imp_less_multiset: "A \<notin> Interp C \<Longrightarrow> A \<in> interp D \<Longrightarrow> C #\<subset># D"
+  using less_eq_imp_interp_subseteq_Interp multiset_linorder.not_less by blast
+
+lemma false_interp_to_true_interp_imp_less_multiset: "A \<notin> interp C \<Longrightarrow> A \<in> interp D \<Longrightarrow> C #\<subset># D"
+  using less_eq_imp_interp_subseteq_interp multiset_linorder.not_less by blast
+
+lemma false_Interp_to_true_Interp_imp_less_multiset: "A \<notin> Interp C \<Longrightarrow> A \<in> Interp D \<Longrightarrow> C #\<subset># D"
+  using less_eq_imp_Interp_subseteq_Interp multiset_linorder.not_less by blast
+
+lemma false_interp_to_true_Interp_imp_le_multiset: "A \<notin> interp C \<Longrightarrow> A \<in> Interp D \<Longrightarrow> C #\<subseteq># D"
+  using less_imp_Interp_subseteq_interp multiset_linorder.not_less by blast
+
+lemma interp_subseteq_INTERP: "interp C \<subseteq> INTERP"
+  unfolding interp_def INTERP_def by (auto simp: production_unfold)
+
+lemma production_subseteq_INTERP: "production C \<subseteq> INTERP"
+  unfolding INTERP_def using production_unfold by blast
+
+lemma Interp_subseteq_INTERP: "Interp C \<subseteq> INTERP"
+  unfolding Interp_def by (auto intro!: interp_subseteq_INTERP production_subseteq_INTERP)
+
+text \<open>This lemma corresponds to \ref{prop:prop:suppmcprop}.\<close>
+lemma produces_imp_in_interp:
+  assumes a_in_c: "Neg A \<in># C" and d: "produces D A"
+  shows "A \<in> interp C"
+proof -
+  from d have "Max (set_mset D) = Pos A"
+    using production_unfold by blast
+  hence "D #\<subset># {#Neg A#}"
+    by (auto intro: Max_pos_neg_less_multiset)
+  moreover have "{#Neg A#} #\<subseteq># C"
+    by (rule less_eq_imp_le_multiset) (rule mset_le_single[OF a_in_c[unfolded mem_set_mset_iff]])
+  ultimately show ?thesis
+    using d by (blast dest: less_eq_imp_interp_subseteq_interp less_imp_production_subseteq_interp)
+qed
+
+lemma neg_notin_Interp_not_produce: "Neg A \<in># C \<Longrightarrow> A \<notin> Interp D \<Longrightarrow> C #\<subseteq># D \<Longrightarrow> \<not> produces D'' A"
+  by (auto dest: produces_imp_in_interp less_eq_imp_interp_subseteq_Interp)
+
+lemma in_production_imp_produces: "A \<in> production C \<Longrightarrow> produces C A"
+  by (metis insert_absorb productive_imp_produces_Max_atom singleton_insert_inj_eq')
+
+lemma not_produces_imp_notin_production: "\<not> produces C A \<Longrightarrow> A \<notin> production C"
+  by (metis in_production_imp_produces)
+
+lemma not_produces_imp_notin_interp: "(\<And>D. \<not> produces D A) \<Longrightarrow> A \<notin> interp C"
+  unfolding interp_def by (fast intro!: in_production_imp_produces)
+
+text {*
+The results below corresponds to Lemma 3.4.
+
+\begin{nit}
+If $D = D'$ and $D$ is productive, $I^D \subseteq I_{D'}$ does not hold. 
+\end{nit}
+*}
+
+lemma true_Interp_imp_general:
+  assumes
+    c_le_d: "C #\<subseteq># D" and
+    d_lt_d': "D #\<subset># D'" and
+    c_at_d: "Interp D \<Turnstile>h C" and
+    subs: "interp D' \<subseteq> (\<Union>C \<in> CC. production C)"
+  shows "(\<Union>C \<in> CC. production C) \<Turnstile>h C"
+proof (cases "\<exists>A. Pos A \<in># C \<and> A \<in> Interp D")
+  case True
+  then obtain A where a_in_c: "Pos A \<in># C" and a_at_d: "A \<in> Interp D"
+    by blast
+  from a_at_d have "A \<in> interp D'"
+    using d_lt_d' less_imp_Interp_subseteq_interp by blast
+  thus ?thesis
+    using subs a_in_c by (blast dest: contra_subsetD)
+next
+  case False
+  then obtain A where a_in_c: "Neg A \<in># C" and "A \<notin> Interp D"
+    using c_at_d unfolding true_cls_def by blast
+  hence "\<And>D''. \<not> produces D'' A"
+    using c_le_d neg_notin_Interp_not_produce by simp
+  thus ?thesis
+    using a_in_c subs not_produces_imp_notin_production by auto
+qed
+
+lemma true_Interp_imp_interp: "C #\<subseteq># D \<Longrightarrow> D #\<subset># D' \<Longrightarrow> Interp D \<Turnstile>h C \<Longrightarrow> interp D' \<Turnstile>h C"
+  using interp_def true_Interp_imp_general by simp
+
+lemma true_Interp_imp_Interp: "C #\<subseteq># D \<Longrightarrow> D #\<subset># D' \<Longrightarrow> Interp D \<Turnstile>h C \<Longrightarrow> Interp D' \<Turnstile>h C"
+  using Interp_as_UNION interp_subseteq_Interp true_Interp_imp_general by simp
+
+lemma true_Interp_imp_INTERP: "C #\<subseteq># D \<Longrightarrow> Interp D \<Turnstile>h C \<Longrightarrow> INTERP \<Turnstile>h C"
+  using INTERP_def interp_subseteq_INTERP
+    true_Interp_imp_general[OF _ less_multiset_right_total]
+  by simp
+
+lemma true_interp_imp_general:
+  assumes
+    c_le_d: "C #\<subseteq># D" and
+    d_lt_d': "D #\<subset># D'" and
+    c_at_d: "interp D \<Turnstile>h C" and
+    subs: "interp D' \<subseteq> (\<Union>C \<in> CC. production C)"
+  shows "(\<Union>C \<in> CC. production C) \<Turnstile>h C"
+proof (cases "\<exists>A. Pos A \<in># C \<and> A \<in> interp D")
+  case True
+  then obtain A where a_in_c: "Pos A \<in># C" and a_at_d: "A \<in> interp D"
+    by blast
+  from a_at_d have "A \<in> interp D'"
+    using d_lt_d' less_eq_imp_interp_subseteq_interp[OF multiset_order.less_imp_le] by blast
+  thus ?thesis
+    using subs a_in_c by (blast dest: contra_subsetD)
+next
+  case False
+  then obtain A where a_in_c: "Neg A \<in># C" and "A \<notin> interp D"
+    using c_at_d unfolding true_cls_def by blast
+  hence "\<And>D''. \<not> produces D'' A"
+    using c_le_d by (auto dest: produces_imp_in_interp less_eq_imp_interp_subseteq_interp)
+  thus ?thesis
+    using a_in_c subs not_produces_imp_notin_production by auto
+qed
+
+text \<open>This lemma corresponds to \ref{prop:prop:suppmcprop}. Here the strict maximality is important\<close>
+lemma true_interp_imp_interp: "C #\<subseteq># D \<Longrightarrow> D #\<subset># D' \<Longrightarrow> interp D \<Turnstile>h C \<Longrightarrow> interp D' \<Turnstile>h C"
+  using interp_def true_interp_imp_general by simp
+
+lemma true_interp_imp_Interp: "C #\<subseteq># D \<Longrightarrow> D #\<subset># D' \<Longrightarrow> interp D \<Turnstile>h C \<Longrightarrow> Interp D' \<Turnstile>h C"
+  using Interp_as_UNION interp_subseteq_Interp[of D'] true_interp_imp_general by simp
+
+lemma true_interp_imp_INTERP: "C #\<subseteq># D \<Longrightarrow> interp D \<Turnstile>h C \<Longrightarrow> INTERP \<Turnstile>h C"
+  using INTERP_def interp_subseteq_INTERP
+    true_interp_imp_general[OF _ less_multiset_right_total]
+  by simp
+
+lemma productive_imp_false_interp: "productive C \<Longrightarrow> \<not> interp C \<Turnstile>h C"
+  unfolding production_unfold by auto
+
+text \<open>This lemma corresponds to \ref{prop:prop:suppmcprop}. Here the strict maximality is important\<close>
+lemma cls_gt_double_pos_no_production:
+  assumes D: "{#Pos P, Pos P#} #\<subset># C"
+  shows "\<not>produces C P"
+proof -
+  let ?D = "{#Pos P, Pos P#}"
+  note D' = D[unfolded less_multiset\<^sub>H\<^sub>O]
+  consider
+    (P) "count C (Pos P) \<ge> 2"
+  | (Q) Q where "Q > Pos P" and "Q \<in># C "
+    using HOL.spec[OF HOL.conjunct2[OF D'], of "Pos P"] by auto 
+  thus ?thesis
+    proof cases
+      case Q
+      have "Q \<in> set_mset C" 
+        using Q(2) by (auto split: split_if_asm)
+      then have "Max (set_mset C) > Pos P"
+        using Q(1) Max_gr_iff by blast
+      thus ?thesis
+        unfolding production_unfold by auto
+    next
+      case P
+      thus ?thesis
+        unfolding production_unfold by auto
+    qed
+qed
+
+
+text \<open>This lemma corresponds to \ref{prop:prop:suppmcprop}.\<close>
+lemma
+  assumes D: "C+{#Neg P#} #\<subset># D" 
+  shows "production D \<noteq> {P}"
+proof -
+  note D' = D[unfolded less_multiset\<^sub>H\<^sub>O]
+  consider
+    (P) "Neg P \<in># D"
+  | (Q) Q where "Q > Neg P" and "count D Q > count (C + {#Neg P#}) Q"
+    using HOL.spec[OF HOL.conjunct2[OF D'], of "Neg P"] by fastforce 
+  thus ?thesis
+    proof cases
+      case Q
+      have "Q \<in> set_mset D" 
+        using Q(2) by (auto split: split_if_asm)
+      then have "Max (set_mset D) > Neg P"
+        using Q(1) Max_gr_iff by blast
+      hence "Max (set_mset D) > Pos P"
+        using less_trans[of "Pos P" "Neg P" "Max (set_mset D)"] by auto
+      thus ?thesis
+        unfolding production_unfold by auto
+    next
+      case P
+      hence "Max (set_mset D) > Pos P"
+        by (meson Max_ge finite_set_mset le_less_trans linorder_not_le mem_set_mset_iff
+          pos_less_neg)
+      thus ?thesis
+        unfolding production_unfold by auto
+    qed
+qed
 
 end
 
-interpretation selection "(\<lambda>_. {#})"
-  by standard auto
+(*TODO sharing with Propo_CDCL*)
+abbreviation "MMax M \<equiv> Max (set_mset M)"
+
+subsection \<open>We can now define the rules of the calculus\<close>
+inductive superposition_rules :: "'a clause \<Rightarrow> 'a clause \<Rightarrow> 'a clause \<Rightarrow> bool" where
+factoring: "superposition_rules (C + {#Pos P#} + {#Pos P#}) B (C + {#Pos P#})" |
+superposition_l: "superposition_rules (C\<^sub>1 + {#Pos P#}) (C\<^sub>2 + {#Pos P#}) (C\<^sub>1+ C\<^sub>2)"
+  
+inductive superposition :: "'a clauses \<Rightarrow> 'a clauses \<Rightarrow> bool" where
+superposition: "A \<in> N \<Longrightarrow> B \<in> N \<Longrightarrow> superposition_rules A B C
+  \<Longrightarrow> superposition N (N \<union> {C})"
+
+end
+definition abstract_red :: "'a::wellorder clause \<Rightarrow> 'a clauses \<Rightarrow> bool" where
+"abstract_red C N = (clss_lt N C \<Turnstile>p C)"
+
+(*TODO: remove when multiset is of sort ord again*)
+instantiation multiset :: (linorder) linorder
+begin
+
+definition less_multiset :: "'a::linorder multiset \<Rightarrow> 'a multiset \<Rightarrow> bool" where
+  "M' < M \<longleftrightarrow> M' #\<subset># M"
+
+definition less_eq_multiset :: "'a multiset \<Rightarrow> 'a multiset \<Rightarrow>bool" where
+   "(M'::'a multiset) \<le> M \<longleftrightarrow> M' #\<subseteq># M"
+
+instance
+  by standard (auto simp add: less_eq_multiset_def less_multiset_def multiset_order.less_le_not_le add.commute multiset_order.add_right_mono)
+end
+
+lemma less_multiset[iff]: "M < N \<longleftrightarrow> M #\<subset># N"
+  unfolding less_multiset_def by auto
+
+lemma less_eq_multiset[iff]: "M \<le> N \<longleftrightarrow> M #\<subseteq># N"
+  unfolding less_eq_multiset_def by auto
+
+lemma herbrand_true_clss_true_clss_cls_herbrand_true_clss:
+  assumes 
+    AB: "A \<Turnstile>hs B" and
+    BC: "B \<Turnstile>p C"
+  shows "A \<Turnstile>h C"
+proof -
+  let ?I = "{Pos P |P. P \<in> A} \<union> {Neg P |P. P \<notin> A}"
+  have B: "?I \<Turnstile>s B" using AB
+    by (auto simp add: herbrand_interp_iff_partial_interp_clss)
+  
+  have IH: "\<And>I. total_over_set I (atms_of C) \<Longrightarrow> total_over_m I B \<Longrightarrow> consistent_interp I \<Longrightarrow> I \<Turnstile>s B \<Longrightarrow> I \<Turnstile> C" using BC
+    by (auto simp add: true_clss_cls_def)
+  show ?thesis
+    unfolding herbrand_interp_iff_partial_interp_cls
+    by (auto intro: IH[of ?I] simp add: herbrand_total_over_set herbrand_total_over_m herbrand_consistent_interp B)
+qed
+  
+  
+  
+locale ground_ordered_resolution_with_redundancy = 
+  ground_resolution_with_selection +
+  fixes redundant :: "'a::wellorder clause \<Rightarrow> 'a clauses \<Rightarrow> bool" 
+  assumes redundant_is_abstract: "redundant A N \<Longrightarrow> abstract_red A N"
+begin
+definition saturated :: "'a clauses \<Rightarrow> bool" where
+"saturated N \<longleftrightarrow> (\<forall>A B C. \<not>redundant A N \<longrightarrow> \<not>redundant B N \<longrightarrow> superposition_rules A B C \<longrightarrow> redundant C N)"
 
 
-interpretation ground_resolution_with_selection "(\<lambda>_. {#})"
-  by standard auto
+lemma
+  assumes "saturated N" and
+  finite: "finite N" and
+  empty: "{#} \<notin> N"
+  shows "INTERP N \<Turnstile>hs N"
+proof (rule ccontr)
+  let ?I = "INTERP N"
+  assume "\<not> ?thesis"
+  hence not_empty: "{E\<in>N. \<not>?I \<Turnstile>h E} \<noteq> {}"
+    unfolding true_clss_def Ball_def by auto
+  let ?D = "Min {E\<in>N. \<not>?I \<Turnstile>h E}"
+  have [simp]: "?D \<in> N" 
+    by (metis (mono_tags, lifting) Min_in not_empty finite mem_Collect_eq rev_finite_subset subsetI)
+  have not_d_interp[simp]: "\<not>?I \<Turnstile>h ?D"
+    by (metis (mono_tags, lifting) Min_in finite mem_Collect_eq not_empty rev_finite_subset subsetI)
+  have cls_not_D: "\<forall>E. E \<in> N \<longrightarrow> E \<noteq> ?D \<longrightarrow> \<not>?I \<Turnstile>h E \<longrightarrow> ?D \<le> E"
+    using finite by (auto simp del: less_eq_multiset)
+  obtain C L where D: "?D = C + {#L#}"  and LSD: "L \<in># S ?D \<or> (S ?D = {#} \<and> Max (set_mset ?D) = L)"
+    proof (cases "S ?D = {#}")
+      case False
+      then obtain L where "L \<in># S ?D"
+        using Max_in_lits by blast
+      moreover 
+        hence "L \<in># ?D"
+          using S_selects_subseteq[of ?D] by auto
+        hence "?D = (?D - {#L#}) + {#L#}"
+          by auto
+      ultimately show ?thesis using that by blast
+    next
+      let ?L = "MMax ?D"
+      case True
+      moreover
+        have "?L \<in># ?D"
+          by (metis (no_types, lifting) Max_in_lits `Min {E \<in> N. \<not> INTERP N \<Turnstile>h E} \<in> N` empty)
+        hence "?D = (?D - {#?L#}) + {#?L#}"
+          by auto
+      ultimately show ?thesis using that by blast
+    qed
+  have red: "\<not>redundant ?D N"
+    proof (rule ccontr)
+      assume red[simplified]: "~~redundant ?D N"
+       
+      have "\<forall>E < ?D. E \<in> N \<longrightarrow> ?I \<Turnstile>h E"
+        using cls_not_D not_le by fastforce
+      hence "?I \<Turnstile>hs clss_lt N ?D"
+        unfolding clss_lt_def true_clss_def Ball_def by blast
+      thus False
+        using redundant_is_abstract[simplified, OF red] not_d_interp unfolding abstract_red_def 
+        using herbrand_true_clss_true_clss_cls_herbrand_true_clss by fast
+    qed
+    
+  consider
+    (L) P where "L = Pos P" and "S ?D = {#}" and "Max (set_mset ?D) = Pos P"
+  | (Lneg) P where "L = Neg P"
+    using LSD S_selects_neg_lits[of ?D L] by (cases L) auto
+  thus False
+    proof cases
+      case L note P = this(1) and S = this(2) and max = this(3)
+      have "count ?D L > 1"
+        proof (rule ccontr)
+          assume "~ ?thesis"
+          hence count: "count ?D L = 1"
+            unfolding D by auto
+            
+          have "produces N ?D P"
+            unfolding production_iff_produces unfolding production_unfold apply (auto simp add: max not_empty)
+            using not_empty empty finite `Min {E \<in> N. \<not> ?I \<Turnstile>h E} \<in> N` apply auto[1]
+            using count L apply auto[1]
+            using not_d_interp true_interp_imp_INTERP ground_resolution_with_selection_axioms 
+              apply blast
+            using S apply auto[1]
+            done
+          hence "INTERP N \<Turnstile>h ?D"
+            unfolding D
+            by (metis pos_literal_in_imp_true_cls produces_imp_Pos_in_lits production_subseteq_INTERP singletonI subsetCE)
+          thus False
+            using not_d_interp by blast
+        qed
+      then obtain C' where C':"?D = C' + {#Pos P#} + {#Pos P#}"
+        unfolding D by (metis P add.left_neutral add_less_cancel_right count_single count_union multi_member_split)
+      have "superposition_rules ?D ?D (?D - {#L#})"
+        unfolding C' L by (auto simp add: superposition_rules.simps) 
+      have "abstract_red (?D - {#L#}) N \<Longrightarrow> abstract_red ?D N" 
+        unfolding C' L abstract_red_def clss_lt_def true_clss_cls_def apply safe
+        sorry
+      have "?D - {#L#} #\<subset># ?D"
+        unfolding C' L by auto
+        
+      show False sorry
+    next
+      case Lneg
+      
+      show False sorry
+  qed
+qed
+    
+end
 
+
+
+
+lemma tautology_is_redundant:
+  assumes "tautology C"
+  shows "abstract_red C N"
+  using assms unfolding abstract_red_def true_clss_cls_def tautology_def by auto
+  
+lemma subsumed_is_redundant:
+  assumes AB: "A \<subset># B"
+  and AN: "A \<in> N" and "B \<in> N"
+  shows "abstract_red B N"
+proof -
+  have "A \<in> clss_lt N B" using AN AB unfolding clss_lt_def 
+    by (auto dest: less_eq_imp_le_multiset simp add: multiset_order.dual_order.order_iff_strict)
+  thus ?thesis
+    using AB unfolding abstract_red_def true_clss_cls_def Partial_Clausal_Logic.true_clss_def by blast
+qed
+
+inductive redundant :: "'a clause \<Rightarrow> 'a clauses \<Rightarrow> bool" where
+subsumption: "A \<subset># B \<Longrightarrow> A \<in> N \<Longrightarrow> B \<in> N \<Longrightarrow> redundant B N"
+
+lemma redundant_is_redundancy_criterion:
+  fixes A :: "'a :: wellorder clause" and N :: "'a :: wellorder clauses"
+  assumes "redundant A N"
+  shows  "abstract_red A N"
+  using assms 
+proof (induction rule: redundant.induct)
+  case (subsumption A B N)
+  thus ?case
+    using subsumed_is_redundant[of A B N] unfolding abstract_red_def clss_lt_def by auto
+qed
+
+locale truc=
+    selection S for S :: "('a :: wellorder) clause \<Rightarrow> 'a clause"
+begin
+
+interpretation truc: ground_ordered_resolution_with_redundancy S redundant
+  using redundant_is_redundancy_criterion by unfold_locales auto
+end
 end
